theories/STLCmu/boring.v
@@ -1,0 +1,636 @@
+(* STLCmu and STLCmuVS are the same thing;
+   this file encodes this truth by a bunch of trivial mappings and lemmas *)
+
+(* trivial embedding from STLCmu into STLCmuVS  *)
+(* -------------------------------------------  *)
+
+From st.STLCmu Require Import lang typing.
+From st.STLCmuVS Require Import lang typing.
+From st.prelude Require Import lang_base.
+
+Reserved Notation "[[ e ]]" (at level 4, e at next level).
+Fixpoint embd_expr (e : STLCmu.lang.expr) : STLCmuVS.lang.expr :=
+  match e with
+  | STLCmu.lang.Var x => Var x
+  | STLCmu.lang.LetIn e1 e2 => LetIn [[e1]] [[e2]]
+  | STLCmu.lang.Lam e => Lam [[e]]
+  | STLCmu.lang.App e1 e2 => App [[e1]] [[e2]]
+  | STLCmu.lang.Lit l => match l with
+                       | LitInt n => n
+                       | LitBool b => b
+                       | LitUnit => ()%Eₙₒ
+                       end
+  | STLCmu.lang.BinOp op e1 e2 => BinOp op [[e1]] [[e2]]
+  | STLCmu.lang.If e0 e1 e2 => If [[e0]] [[e1]] [[e2]]
+  | STLCmu.lang.Seq e1 e2 => Seq [[e1]] [[e2]]
+  | STLCmu.lang.Pair e1 e2 => Pair [[e1]] [[e2]]
+  | STLCmu.lang.Fst e => Fst [[e]]
+  | STLCmu.lang.Snd e => Snd [[e]]
+  | STLCmu.lang.InjL e => InjL [[e]]
+  | STLCmu.lang.InjR e => InjR [[e]]
+  | STLCmu.lang.Case e0 e1 e2 => Case [[e0]] [[e1]] [[e2]]
+  | STLCmu.lang.Fold e => Fold [[e]]
+  | STLCmu.lang.Unfold e => Unfold [[e]]
+  end
+where "[[ e ]]" := (embd_expr e).
+
+Lemma embd_expr_ren e :
+  forall k l, [[ e.[upn l (ren (+k))] ]] = [[e]].[upn l (ren (+k))].
+Proof.
+  induction e; intros k m; asimpl.
+  - do 2 rewrite (iter_up m x (ren (+k))).
+    destruct (lt_dec x m); by asimpl.
+  - erewrite IHe0. by erewrite IHe.
+  - by erewrite IHe.
+  - erewrite IHe1. by erewrite IHe2.
+  - by destruct l.
+  - erewrite IHe1. by erewrite IHe2.
+  - erewrite IHe1. erewrite IHe2. by erewrite IHe3.
+  - erewrite IHe1. by erewrite IHe2.
+  - erewrite IHe1. by erewrite IHe2.
+  - by erewrite IHe.
+  - by erewrite IHe.
+  - by erewrite IHe.
+  - by erewrite IHe.
+  - erewrite IHe. erewrite IHe0. by erewrite IHe1.
+  - by erewrite IHe.
+  - by erewrite IHe.
+Qed.
+
+Lemma comm_embd_expr_subst_gen e e' : ∀ n, [[e.[upn n (e' .: ids)] ]] = [[e]].[upn n ([[e']] .: ids)].
+Proof.
+  induction e; intros n; asimpl.
+  - rewrite (iter_up n x (e' .: ids)) (iter_up n x ([[e']] .: ids)).
+    destruct (lt_dec x n).
+      + by asimpl.
+      + destruct (decide (x - n = 0)); asimpl. rewrite e. asimpl.
+        cut ([[ e'.[upn 0 (ren (+n))] ]] = ([[ e' ]]).[upn 0 (ren (+n))]).
+        by asimpl. by rewrite embd_expr_ren.
+        destruct (x - n). exfalso; lia. by asimpl.
+  - erewrite IHe. by erewrite IHe0.
+  - by erewrite IHe.
+  - erewrite IHe1. by erewrite IHe2.
+  - by destruct l.
+  - erewrite IHe1. by erewrite IHe2.
+  - erewrite IHe1. erewrite IHe2. by erewrite IHe3.
+  - erewrite IHe1. by erewrite IHe2.
+  - erewrite IHe1. by erewrite IHe2.
+  - by erewrite IHe.
+  - by erewrite IHe.
+  - by erewrite IHe.
+  - by erewrite IHe.
+  - erewrite IHe. erewrite IHe0. by erewrite IHe1.
+  - by erewrite IHe.
+  - by erewrite IHe.
+Qed.
+
+Lemma comm_embd_expr_subst e e' : [[e.[e'/]]] = [[e]].[[[e']]/].
+Proof.
+  cut ([[e.[upn 0 (e' .: ids)] ]] = ([[e]]).[upn 0 ([[e']] .: ids)]); [by asimpl|].
+  apply comm_embd_expr_subst_gen.
+Qed.
+
+Fixpoint embd_val (v : STLCmu.lang.val) : STLCmuVS.lang.val :=
+  match v with
+  | STLCmu.lang.LamV e => LamV (embd_expr e)
+  | STLCmu.lang.LitV v => LitV v
+  | STLCmu.lang.PairV v1 v2 => PairV (embd_val v1) (embd_val v2)
+  | STLCmu.lang.InjLV v => InjLV (embd_val v)
+  | STLCmu.lang.InjRV v => InjRV (embd_val v)
+  | STLCmu.lang.FoldV v => FoldV (embd_val v)
+  end.
+
+Lemma to_val_embd_expr e : to_val (embd_expr e) = (STLCmu.lang.to_val e) ≫= (fun v => Some (embd_val v)).
+Proof.
+  induction e; simplify_option_eq; try done.
+  - by destruct l.
+  - simpl. rewrite IHe1 IHe2. simplify_option_eq.
+    destruct (STLCmu.lang.to_val e1) eqn:eq1.
+    + simplify_option_eq. destruct (STLCmu.lang.to_val e2) eqn:eq2; by simplify_option_eq.
+    + by simplify_option_eq.
+  - rewrite IHe. simplify_option_eq.
+    destruct (STLCmu.lang.to_val e) eqn:eq; by simplify_option_eq.
+  - rewrite IHe. simplify_option_eq.
+    destruct (STLCmu.lang.to_val e) eqn:eq; by simplify_option_eq.
+  - rewrite IHe. simplify_option_eq.
+    destruct (STLCmu.lang.to_val e) eqn:eq; by simplify_option_eq.
+Qed.
+
+Lemma of_val_embd_expr v : of_val (embd_val v) = embd_expr (STLCmu.lang.of_val v).
+Proof.
+  induction v; simpl; try by rewrite IHv. done. by destruct v. by rewrite IHv1 IHv2. Qed.
+
+Lemma embd_expr_typed Γ (e : STLCmu.lang.expr) τ (de : STLCmu.typing.typed Γ e τ) :
+  STLCmuVS.typing.typed Γ (embd_expr e) τ.
+Proof. induction de; try by repeat econstructor. Qed.
+
+From st.STLCmu Require Import contexts.
+From st.STLCmuVS Require Import contexts.
+
+Definition embd_ctx_item (Ci : STLCmu.contexts.ctx_item) : STLCmuVS.contexts.ctx_item :=
+  match Ci with
+  | STLCmu.contexts.CTX_Lam => CTX_Lam
+  | STLCmu.contexts.CTX_AppL e2 => CTX_AppL [[e2]]
+  | STLCmu.contexts.CTX_AppR e1 => CTX_AppR [[e1]]
+  | STLCmu.contexts.CTX_LetInL e2 => CTX_LetInL [[e2]]
+  | STLCmu.contexts.CTX_LetInR e1 => CTX_LetInR [[e1]]
+  | STLCmu.contexts.CTX_PairL e2 => CTX_PairL [[e2]]
+  | STLCmu.contexts.CTX_PairR e1 => CTX_PairR [[e1]]
+  | STLCmu.contexts.CTX_Fst => CTX_Fst
+  | STLCmu.contexts.CTX_Snd => CTX_Snd
+  | STLCmu.contexts.CTX_InjL => CTX_InjL
+  | STLCmu.contexts.CTX_InjR => CTX_InjR
+  | STLCmu.contexts.CTX_CaseL e1 e2 => CTX_CaseL [[e1]] [[e2]]
+  | STLCmu.contexts.CTX_CaseM e0 e2 => CTX_CaseM [[e0]] [[e2]]
+  | STLCmu.contexts.CTX_CaseR e0 e1 => CTX_CaseR [[e0]] [[e1]]
+  | STLCmu.contexts.CTX_BinOpL op e2 => CTX_BinOpL op [[e2]]
+  | STLCmu.contexts.CTX_BinOpR op e1 => CTX_BinOpR op [[e1]]
+  | STLCmu.contexts.CTX_IfL e1 e2 => CTX_IfL [[e1]] [[e2]]
+  | STLCmu.contexts.CTX_IfM e0 e2 => CTX_IfM [[e0]] [[e2]]
+  | STLCmu.contexts.CTX_IfR e0 e1 => CTX_IfR [[e0]] [[e1]]
+  | STLCmu.contexts.CTX_Fold => CTX_Fold
+  | STLCmu.contexts.CTX_Unfold => CTX_Unfold
+  end.
+
+Definition embd_ctx (C : STLCmu.contexts.ctx) : STLCmuVS.contexts.ctx :=
+  fmap embd_ctx_item C.
+
+Lemma comm_embd_fill_ctx_item Ci e :
+  STLCmuVS.contexts.fill_ctx_item (embd_ctx_item Ci) (embd_expr e) =
+  embd_expr (STLCmu.contexts.fill_ctx_item Ci e).
+Proof. destruct Ci; by simpl. Qed.
+
+Lemma comm_embd_fill_ctx C e :
+  STLCmuVS.contexts.fill_ctx (embd_ctx C) (embd_expr e) =
+  embd_expr (STLCmu.contexts.fill_ctx C e).
+Proof. induction C; simpl; try done. rewrite IHC. erewrite comm_embd_fill_ctx_item; eauto. Qed.
+
+From st.STLCmu Require Import reducibility.
+From st.STLCmuVS Require Import reducibility.
+
+Lemma embd_expr_Reducible (e : STLCmu.lang.expr) (de : STLCmu.reducibility.Reducible e) :
+  STLCmuVS.reducibility.Reducible (embd_expr e).
+Proof.
+  induction de; intros; simpl; try by econstructor.
+  - eapply LetIn_D_Red. by rewrite to_val_embd_expr H.
+  - eapply App_R_Red; auto. by rewrite to_val_embd_expr H.
+  - eapply App_D_Red; auto. by rewrite to_val_embd_expr H.
+  - eapply BinOp_R_Red; auto. by rewrite to_val_embd_expr H.
+  - eapply Pair_R_Red; auto. by rewrite to_val_embd_expr H.
+  - eapply Fst_D_Red; auto. by rewrite to_val_embd_expr H. by rewrite to_val_embd_expr H0.
+  - eapply Snd_D_Red; auto. by rewrite to_val_embd_expr H. by rewrite to_val_embd_expr H0.
+  - eapply Case_D_InjL_Red; auto. by rewrite to_val_embd_expr H.
+  - eapply Case_D_InjR_Red; auto. by rewrite to_val_embd_expr H.
+  - eapply Unfold_D_Red; auto. by rewrite to_val_embd_expr H.
+Qed.
+
+Lemma embd_expr_head_step_help (e : STLCmu.lang.expr) (e' : STLCmu.lang.expr) :
+  STLCmu_head_step e e' → STLCmuVS_head_step (embd_expr e) (embd_expr e').
+Proof.
+  intro Hstep. destruct Hstep; simpl; try by econstructor.
+  - rewrite comm_embd_expr_subst. econstructor. rewrite to_val_embd_expr H. by simplify_option_eq.
+  - rewrite comm_embd_expr_subst. econstructor. rewrite to_val_embd_expr H. by simplify_option_eq.
+  - rewrite -(STLCmu.lang.of_to_val _ _ H) -(STLCmu.lang.of_to_val _ _ H0). rewrite -!of_val_embd_expr /=.
+    replace (STLCmuVS.lang.of_val (embd_val (STLCmu.lang.bin_op_eval op z1 z2))) with
+        (of_val (bin_op_eval op z1 z2)) by by destruct op.
+    by econstructor.
+  - rewrite -(STLCmu.lang.of_to_val _ _ H) /=. by econstructor.
+  - econstructor. by rewrite to_val_embd_expr H /=. by rewrite to_val_embd_expr H0 /=.
+  - econstructor. by rewrite to_val_embd_expr H /=. by rewrite to_val_embd_expr H0 /=.
+  - rewrite -(STLCmu.lang.of_to_val _ _ H) /= -of_val_embd_expr comm_embd_expr_subst of_val_embd_expr.
+    econstructor. by rewrite to_val_embd_expr STLCmu.lang.to_of_val /=.
+  - rewrite -(STLCmu.lang.of_to_val _ _ H) /= -of_val_embd_expr comm_embd_expr_subst of_val_embd_expr.
+    econstructor. by rewrite to_val_embd_expr STLCmu.lang.to_of_val /=.
+  - econstructor. by rewrite to_val_embd_expr H /=.
+Qed.
+
+Definition embd_ectx_item (Ki : STLCmu.lang.ectx_item) : STLCmuVS.lang.ectx_item :=
+  match Ki with
+  | STLCmu.lang.LetInCtx e2 => LetInCtx [[e2]]
+  | STLCmu.lang.AppLCtx e2 => AppLCtx [[e2]]
+  | STLCmu.lang.AppRCtx v1 => AppRCtx (embd_val v1)
+  | STLCmu.lang.PairLCtx e2 => PairLCtx [[e2]]
+  | STLCmu.lang.PairRCtx v1 => PairRCtx (embd_val v1)
+  | STLCmu.lang.FstCtx => FstCtx
+  | STLCmu.lang.SndCtx => SndCtx
+  | STLCmu.lang.InjLCtx => InjLCtx
+  | STLCmu.lang.InjRCtx => InjRCtx
+  | STLCmu.lang.CaseCtx e1 e2 => CaseCtx [[e1]] [[e2]]
+  | STLCmu.lang.IfCtx e2 e3 => IfCtx [[e2]] [[e3]]
+  | STLCmu.lang.BinOpLCtx op e2 => BinOpLCtx op [[e2]]
+  | STLCmu.lang.BinOpRCtx op v1 => BinOpRCtx op (embd_val v1)
+  | STLCmu.lang.SeqCtx e2 => SeqCtx [[e2]]
+  | STLCmu.lang.FoldCtx => FoldCtx
+  | STLCmu.lang.UnfoldCtx => UnfoldCtx
+  end.
+
+Definition embd_ectx (K : list STLCmu.lang.ectx_item) : (list STLCmuVS.lang.ectx_item) :=
+  fmap embd_ectx_item K.
+
+Lemma comm_embd_fill_ectx_item Ki e :
+  STLCmuVS.lang.fill_item (embd_ectx_item Ki) (embd_expr e) =
+  embd_expr (STLCmu.lang.fill_item Ki e).
+Proof. destruct Ki; simpl; try done; by rewrite of_val_embd_expr. Qed.
+
+Lemma comm_embd_fill_ectx K e :
+  fill (embd_ectx K) (embd_expr e) = embd_expr (fill K e).
+Proof.
+  induction K as [|Ki K IHK] using rev_ind; simpl; try done.
+  replace (embd_ectx (K ++ [Ki])) with (embd_ectx K ++ [embd_ectx_item Ki]) by (rewrite /embd_ectx fmap_app; done).
+  by rewrite !fill_app IHK /= comm_embd_fill_ectx_item.
+Qed.
+
+Lemma embd_expr_step_help (e : STLCmu.lang.expr) (e' : STLCmu.lang.expr) :
+  STLCmu_step e e' → STLCmuVS_step (embd_expr e) (embd_expr e').
+Proof.
+  intro Hstep. destruct Hstep. subst. simpl.
+  rewrite -!comm_embd_fill_ectx.
+  apply STLCmuVS_step_ctx. apply (@ectx_lang_ctx STLCmuVS_ectx_lang).
+  by apply head_prim_step, embd_expr_head_step_help.
+Qed.
+
+Lemma embd_expr_step (e : STLCmu.lang.expr) :
+  ∀ (e' : STLCmu.lang.expr), STLCmu_step e e' → STLCmuVS_step (embd_expr e) (embd_expr e').
+Proof.
+  intros e' Hstep.
+  cut (Reducible [[e]]).
+  { intro red. pose proof (iffRL (Reducible_valid _) red).
+    pose proof (iffRL (STLCmuVS_prim_red _) H).
+    destruct H0 as [e'' Hstep'].
+    by apply embd_expr_step_help.
+  }
+  apply embd_expr_Reducible.
+  apply STLCmu.reducibility.Reducible_valid.
+  apply STLCmu_prim_red. by exists e'.
+Qed.
+
+Lemma embd_expr_halts (e : STLCmu.lang.expr) :
+  STLCmu_halts e → STLCmuVS_halts (embd_expr e).
+Proof.
+  intros halts. destruct halts as [v Hrtc].
+  exists (embd_val v). rewrite of_val_embd_expr.
+  eapply rtc_congruence; eauto. apply embd_expr_step.
+Qed.
+
+(* trivial projection from STLCmuVS into STLCmu  *)
+(* --------------------------------------------  *)
+
+From st.STLCmuVS Require Import lang.
+From st.STLCmu Require Import lang.
+From st.prelude Require Import lang_base.
+
+Reserved Notation "<< e >>" (at level 4, e at next level).
+Fixpoint proj_expr (e : STLCmuVS.lang.expr) : STLCmu.lang.expr :=
+  match e with
+  | STLCmuVS.lang.Var x => Var x
+  | STLCmuVS.lang.LetIn e1 e2 => LetIn <<e1>> <<e2>>
+  | STLCmuVS.lang.Lam e => Lam <<e>>
+  | STLCmuVS.lang.App e1 e2 => App <<e1>> <<e2>>
+  | STLCmuVS.lang.Lit l => match l with
+                       | LitInt n => Lit (LitInt n)
+                       | LitBool b => Lit (LitBool b)
+                       | LitUnit => Lit LitUnit
+                       end
+  | STLCmuVS.lang.BinOp op e1 e2 => BinOp op <<e1>> <<e2>>
+  | STLCmuVS.lang.If e0 e1 e2 => If <<e0>> <<e1>> <<e2>>
+  | STLCmuVS.lang.Seq e1 e2 => Seq <<e1>> <<e2>>
+  | STLCmuVS.lang.Pair e1 e2 => Pair <<e1>> <<e2>>
+  | STLCmuVS.lang.Fst e => Fst <<e>>
+  | STLCmuVS.lang.Snd e => Snd <<e>>
+  | STLCmuVS.lang.InjL e => InjL <<e>>
+  | STLCmuVS.lang.InjR e => InjR <<e>>
+  | STLCmuVS.lang.Case e0 e1 e2 => Case <<e0>> <<e1>> <<e2>>
+  | STLCmuVS.lang.Fold e => Fold <<e>>
+  | STLCmuVS.lang.Unfold e => Unfold <<e>>
+  | STLCmuVS.lang.VirtStep e => (Seq (Lit LitUnit) (Lit LitUnit)) (* just a dummy value *)
+  end
+where "<< e >>" := (proj_expr e).
+
+Lemma retraction (e : STLCmu.lang.expr) : proj_expr (embd_expr e) = e.
+Proof.
+  induction e; simpl; try done; try destruct (_ : base_lit); (repeat f_equiv; auto).
+Qed.
+
+From st.STLCmuVS Require Import contexts.
+From st.STLCmu Require Import contexts.
+
+Definition proj_ctx_item (Ci : STLCmuVS.contexts.ctx_item) : STLCmu.contexts.ctx_item :=
+  match Ci with
+  | STLCmuVS.contexts.CTX_Lam => CTX_Lam
+  | STLCmuVS.contexts.CTX_AppL e2 => CTX_AppL <<e2>>
+  | STLCmuVS.contexts.CTX_AppR e1 => CTX_AppR <<e1>>
+  | STLCmuVS.contexts.CTX_LetInL e2 => CTX_LetInL <<e2>>
+  | STLCmuVS.contexts.CTX_LetInR e1 => CTX_LetInR <<e1>>
+  | STLCmuVS.contexts.CTX_PairL e2 => CTX_PairL <<e2>>
+  | STLCmuVS.contexts.CTX_PairR e1 => CTX_PairR <<e1>>
+  | STLCmuVS.contexts.CTX_Fst => CTX_Fst
+  | STLCmuVS.contexts.CTX_Snd => CTX_Snd
+  | STLCmuVS.contexts.CTX_InjL => CTX_InjL
+  | STLCmuVS.contexts.CTX_InjR => CTX_InjR
+  | STLCmuVS.contexts.CTX_CaseL e1 e2 => CTX_CaseL <<e1>> <<e2>>
+  | STLCmuVS.contexts.CTX_CaseM e0 e2 => CTX_CaseM <<e0>> <<e2>>
+  | STLCmuVS.contexts.CTX_CaseR e0 e1 => CTX_CaseR <<e0>> <<e1>>
+  | STLCmuVS.contexts.CTX_BinOpL op e2 => CTX_BinOpL op <<e2>>
+  | STLCmuVS.contexts.CTX_BinOpR op e1 => CTX_BinOpR op <<e1>>
+  | STLCmuVS.contexts.CTX_IfL e1 e2 => CTX_IfL <<e1>> <<e2>>
+  | STLCmuVS.contexts.CTX_IfM e0 e2 => CTX_IfM <<e0>> <<e2>>
+  | STLCmuVS.contexts.CTX_IfR e0 e1 => CTX_IfR <<e0>> <<e1>>
+  | STLCmuVS.contexts.CTX_Fold => CTX_Fold
+  | STLCmuVS.contexts.CTX_Unfold => CTX_Unfold
+  | STLCmuVS.contexts.CTX_VirtStep => CTX_Lam (* just a dummy value *)
+  end.
+
+Definition proj_ctx (C : STLCmuVS.contexts.ctx) : STLCmu.contexts.ctx :=
+  fmap proj_ctx_item C.
+
+From st.STLCmuVS Require Import lang typing reducibility.
+From st.STLCmu Require Import types lang typing.
+From st.prelude Require Import lang_base.
+
+Lemma proj_expr_typed Γ (e : STLCmuVS.lang.expr) τ (de : STLCmuVS.typing.typed Γ e τ) :
+  STLCmu.typing.typed Γ (proj_expr e) τ.
+Proof. induction de; try by repeat econstructor. Qed.
+
+Lemma proj_expr_ren e :
+  forall k l, << e.[upn l (ren (+k))] >> = <<e>>.[upn l (ren (+k))].
+Proof.
+  induction e; intros k m; asimpl.
+  - do 2 rewrite (iter_up m x (ren (+k))).
+    destruct (lt_dec x m); by asimpl.
+  - erewrite IHe0. by erewrite IHe.
+  - by erewrite IHe.
+  - erewrite IHe1. by erewrite IHe2.
+  - by destruct l.
+  - erewrite IHe1. by erewrite IHe2.
+  - erewrite IHe1. erewrite IHe2. by erewrite IHe3.
+  - erewrite IHe1. by erewrite IHe2.
+  - erewrite IHe1. by erewrite IHe2.
+  - by erewrite IHe.
+  - by erewrite IHe.
+  - by erewrite IHe.
+  - by erewrite IHe.
+  - erewrite IHe. erewrite IHe0. by erewrite IHe1.
+  - by erewrite IHe.
+  - by erewrite IHe.
+  - done.
+Qed.
+
+Lemma comm_proj_expr_subst_gen e e' : ∀ n, <<e.[upn n (e' .: ids)] >> = <<e>>.[upn n (<<e'>> .: ids)].
+Proof.
+  induction e; intros n; asimpl.
+  - rewrite (iter_up n x (e' .: ids)) (iter_up n x (<<e'>> .: ids)).
+    destruct (lt_dec x n).
+      + by asimpl.
+      + destruct (decide (x - n = 0)); asimpl. rewrite e. asimpl.
+        cut (<< e'.[upn 0 (ren (+n))] >> = (<< e' >>).[upn 0 (ren (+n))]).
+        by asimpl. by rewrite proj_expr_ren.
+        destruct (x - n). exfalso; lia. by asimpl.
+  - erewrite IHe. by erewrite IHe0.
+  - by erewrite IHe.
+  - erewrite IHe1. by erewrite IHe2.
+  - by destruct l.
+  - erewrite IHe1. by erewrite IHe2.
+  - erewrite IHe1. erewrite IHe2. by erewrite IHe3.
+  - erewrite IHe1. by erewrite IHe2.
+  - erewrite IHe1. by erewrite IHe2.
+  - by erewrite IHe.
+  - by erewrite IHe.
+  - by erewrite IHe.
+  - by erewrite IHe.
+  - erewrite IHe. erewrite IHe0. by erewrite IHe1.
+  - by erewrite IHe.
+  - by erewrite IHe.
+  - done.
+Qed.
+
+Lemma comm_proj_expr_subst e e' : <<e.[e'/]>> = <<e>>.[<<e'>>/].
+Proof.
+  cut (<<e.[upn 0 (e' .: ids)] >> = (<<e>>).[upn 0 (<<e'>> .: ids)]); [by asimpl|].
+  apply comm_proj_expr_subst_gen.
+Qed.
+
+Fixpoint proj_val (v : STLCmuVS.lang.val) : STLCmu.lang.val :=
+  match v with
+  | STLCmuVS.lang.LamV e => LamV (proj_expr e)
+  | STLCmuVS.lang.LitV v => LitV v
+  | STLCmuVS.lang.PairV v1 v2 => PairV (proj_val v1) (proj_val v2)
+  | STLCmuVS.lang.InjLV v => InjLV (proj_val v)
+  | STLCmuVS.lang.InjRV v => InjRV (proj_val v)
+  | STLCmuVS.lang.FoldV v => FoldV (proj_val v)
+  end.
+
+Lemma to_val_proj_expr e : to_val (proj_expr e) = (STLCmuVS.lang.to_val e) ≫= (fun v => Some (proj_val v)).
+Proof.
+  induction e; simplify_option_eq; try done.
+  - by destruct l.
+  - simpl. rewrite IHe1 IHe2. simplify_option_eq.
+    destruct (STLCmuVS.lang.to_val e1) eqn:eq1.
+    + simplify_option_eq. destruct (STLCmuVS.lang.to_val e2) eqn:eq2; by simplify_option_eq.
+    + by simplify_option_eq.
+  - rewrite IHe. simplify_option_eq.
+    destruct (STLCmuVS.lang.to_val e) eqn:eq; by simplify_option_eq.
+  - rewrite IHe. simplify_option_eq.
+    destruct (STLCmuVS.lang.to_val e) eqn:eq; by simplify_option_eq.
+  - rewrite IHe. simplify_option_eq.
+    destruct (STLCmuVS.lang.to_val e) eqn:eq; by simplify_option_eq.
+Qed.
+
+Lemma of_val_proj_expr v : of_val (proj_val v) = proj_expr (STLCmuVS.lang.of_val v).
+Proof.
+  induction v; simpl; try by rewrite IHv. done. by destruct v. by rewrite IHv1 IHv2. Qed.
+
+Lemma proj_ctx_item_typed Γ τ Γ' τ'
+      (Ci : STLCmuVS.contexts.ctx_item) (pCi : STLCmuVS.contexts.typed_ctx_item Ci Γ τ Γ' τ') :
+  STLCmu.contexts.typed_ctx_item (proj_ctx_item Ci) Γ τ Γ' τ'.
+Proof. induction pCi; repeat econstructor; by eapply proj_expr_typed. Qed.
+
+Lemma proj_ctx_typed Γ τ Γ' τ'
+      (C : STLCmuVS.contexts.ctx) (pC : STLCmuVS.contexts.typed_ctx C Γ τ Γ' τ') :
+  STLCmu.contexts.typed_ctx (proj_ctx C) Γ τ Γ' τ'.
+Proof. induction pC; repeat econstructor. by apply proj_ctx_item_typed. apply IHpC. Qed.
+
+Lemma comm_proj_fill_ctx_item Ci Γ τ Γ' τ' (dCi : STLCmuVS.contexts.typed_ctx_item Ci Γ τ Γ' τ') e :
+  STLCmu.contexts.fill_ctx_item (proj_ctx_item Ci) (proj_expr e) =
+  proj_expr (STLCmuVS.contexts.fill_ctx_item Ci e).
+Proof. destruct dCi; by simpl. Qed.
+
+Lemma comm_proj_fill_ctx C Γ τ Γ' τ' (dC : STLCmuVS.contexts.typed_ctx C Γ τ Γ' τ') e :
+  STLCmu.contexts.fill_ctx (proj_ctx C) (proj_expr e) =
+  proj_expr (STLCmuVS.contexts.fill_ctx C e).
+Proof. induction dC; simpl; try done. rewrite IHdC. erewrite comm_proj_fill_ctx_item; eauto. Qed.
+
+From st.STLCmuVS Require Import reducibility.
+From st.STLCmu Require Import reducibility.
+
+Lemma proj_expr_Reducible (e : STLCmuVS.lang.expr) (de : STLCmuVS.reducibility.Reducible e) :
+  STLCmu.reducibility.Reducible (proj_expr e).
+Proof.
+  induction de; intros; simpl; try by econstructor.
+  - eapply LetIn_D_Red. by rewrite to_val_proj_expr H.
+  - eapply App_R_Red; auto. by rewrite to_val_proj_expr H.
+  - eapply App_D_Red; auto. by rewrite to_val_proj_expr H.
+  - eapply BinOp_R_Red; auto. by rewrite to_val_proj_expr H.
+  - eapply Pair_R_Red; auto. by rewrite to_val_proj_expr H.
+  - eapply Fst_D_Red; auto. by rewrite to_val_proj_expr H. by rewrite to_val_proj_expr H0.
+  - eapply Snd_D_Red; auto. by rewrite to_val_proj_expr H. by rewrite to_val_proj_expr H0.
+  - eapply Case_D_InjL_Red; auto. by rewrite to_val_proj_expr H.
+  - eapply Case_D_InjR_Red; auto. by rewrite to_val_proj_expr H.
+  - eapply Unfold_D_Red; auto. by rewrite to_val_proj_expr H.
+Qed.
+
+Lemma proj_expr_head_step_help (e : STLCmuVS.lang.expr) Γ τ (de : STLCmuVS.typing.typed Γ e τ) (e' : STLCmuVS.lang.expr) :
+  STLCmuVS_head_step e e' → STLCmu_head_step (proj_expr e) (proj_expr e').
+Proof.
+  intro Hstep. destruct Hstep; simpl; (try by econstructor); (try by inversion de).
+  - rewrite comm_proj_expr_subst. econstructor. rewrite to_val_proj_expr H. by simplify_option_eq.
+  - rewrite comm_proj_expr_subst. econstructor. rewrite to_val_proj_expr H. by simplify_option_eq.
+  - rewrite -(STLCmuVS.lang.of_to_val _ _ H) -(STLCmuVS.lang.of_to_val _ _ H0). rewrite -!of_val_proj_expr /=.
+    replace (STLCmu.lang.of_val (proj_val (STLCmuVS.lang.bin_op_eval op z1 z2))) with
+        (of_val (bin_op_eval op z1 z2)) by by destruct op.
+    by econstructor.
+  - rewrite -(STLCmuVS.lang.of_to_val _ _ H) /=. by econstructor.
+  - econstructor. by rewrite to_val_proj_expr H /=. by rewrite to_val_proj_expr H0 /=.
+  - econstructor. by rewrite to_val_proj_expr H /=. by rewrite to_val_proj_expr H0 /=.
+  - rewrite -(STLCmuVS.lang.of_to_val _ _ H) /= -of_val_proj_expr comm_proj_expr_subst of_val_proj_expr.
+    econstructor. by rewrite to_val_proj_expr STLCmuVS.lang.to_of_val /=.
+  - rewrite -(STLCmuVS.lang.of_to_val _ _ H) /= -of_val_proj_expr comm_proj_expr_subst of_val_proj_expr.
+    econstructor. by rewrite to_val_proj_expr STLCmuVS.lang.to_of_val /=.
+  - econstructor. by rewrite to_val_proj_expr H /=.
+Qed.
+
+Definition proj_ectx_item (Ki : STLCmuVS.lang.ectx_item) : STLCmu.lang.ectx_item :=
+  match Ki with
+  | STLCmuVS.lang.LetInCtx e2 => LetInCtx <<e2>>
+  | STLCmuVS.lang.AppLCtx e2 => AppLCtx <<e2>>
+  | STLCmuVS.lang.AppRCtx v1 => AppRCtx (proj_val v1)
+  | STLCmuVS.lang.PairLCtx e2 => PairLCtx <<e2>>
+  | STLCmuVS.lang.PairRCtx v1 => PairRCtx (proj_val v1)
+  | STLCmuVS.lang.FstCtx => FstCtx
+  | STLCmuVS.lang.SndCtx => SndCtx
+  | STLCmuVS.lang.InjLCtx => InjLCtx
+  | STLCmuVS.lang.InjRCtx => InjRCtx
+  | STLCmuVS.lang.CaseCtx e1 e2 => CaseCtx <<e1>> <<e2>>
+  | STLCmuVS.lang.IfCtx e2 e3 => IfCtx <<e2>> <<e3>>
+  | STLCmuVS.lang.BinOpLCtx op e2 => BinOpLCtx op <<e2>>
+  | STLCmuVS.lang.BinOpRCtx op v1 => BinOpRCtx op (proj_val v1)
+  | STLCmuVS.lang.SeqCtx e2 => SeqCtx <<e2>>
+  | STLCmuVS.lang.FoldCtx => FoldCtx
+  | STLCmuVS.lang.UnfoldCtx => UnfoldCtx
+  | STLCmuVS.lang.VirtStepCtx => UnfoldCtx
+  end.
+
+Definition proj_ectx (K : list STLCmuVS.lang.ectx_item) : (list STLCmu.lang.ectx_item) :=
+  fmap proj_ectx_item K.
+
+Lemma comm_proj_fill_ectx_item Ki (pKi : Ki ≠ VirtStepCtx) e :
+  STLCmu.lang.fill_item (proj_ectx_item Ki) (proj_expr e) =
+  proj_expr (STLCmuVS.lang.fill_item Ki e).
+Proof. destruct Ki; simpl; try done; by rewrite of_val_proj_expr. Qed.
+
+Lemma comm_proj_fill_ectx K (pK : Forall (fun Ki => Ki ≠ VirtStepCtx) K) e :
+  fill (proj_ectx K) (proj_expr e) = proj_expr (fill K e).
+Proof.
+  revert pK.
+  induction K as [|Ki K IHK] using rev_ind; simpl; try done. intro pK.
+  destruct (iffLR (Forall_app _ _ _) pK) as [pK' pKi]. inversion_clear pKi.
+  replace (proj_ectx (K ++ [Ki])) with (proj_ectx K ++ [proj_ectx_item Ki]) by (rewrite /proj_ectx fmap_app; done). specialize (IHK pK').
+  rewrite !fill_app IHK /= comm_proj_fill_ectx_item; auto.
+Qed.
+
+Lemma blaa K : ∀ Γ e τ, STLCmuVS.typing.typed Γ (fill K e) τ → ∃ Γ' τ', STLCmuVS.typing.typed Γ' e τ'.
+Proof.
+  induction K as [|Ki K IHK] using rev_ind; intros; simpl in *.
+  - by repeat eexists.
+  - rewrite fill_app in H.
+    destruct Ki; inversion H; subst; (try by inversion H0); by eapply IHK.
+Qed.
+
+Lemma blaa' K : ∀ Γ e τ, STLCmuVS.typing.typed Γ (fill K e) τ → Forall (λ Ki : lang.ectx_item, Ki ≠ VirtStepCtx) K.
+Proof.
+  induction K as [|Ki K IHK] using rev_ind; intros; simpl in *; try done.
+  rewrite fill_app in H. apply Forall_app.
+  destruct Ki; inversion H; subst; (try by inversion H0); (by split; [eapply IHK|auto]).
+Qed.
+
+Lemma proj_expr_step_help (e : STLCmuVS.lang.expr) Γ τ (de : STLCmuVS.typing.typed Γ e τ)
+      (e' : STLCmuVS.lang.expr) :
+  STLCmuVS_step e e' → STLCmu_step (proj_expr e) (proj_expr e').
+Proof.
+  intro Hstep. destruct Hstep. subst. simpl.
+  rewrite -!comm_proj_fill_ectx.
+  apply STLCmu_step_ctx. apply (@ectx_lang_ctx STLCmu_ectx_lang).
+  eapply head_prim_step.
+  destruct (blaa _ _ _ _ de) as (Γ' & τ' & de').
+  by eapply proj_expr_head_step_help.
+  eapply blaa', de.
+  eapply blaa', de.
+Qed.
+
+Lemma proj_expr_step (e : STLCmuVS.lang.expr) Γ τ (de : STLCmuVS.typing.typed Γ e τ):
+  ∀ (e' : STLCmuVS.lang.expr), STLCmuVS_step e e' → STLCmu_step (proj_expr e) (proj_expr e').
+Proof.
+  intros e' Hstep.
+  cut (Reducible <<e>>).
+  { intro red. pose proof (iffRL (Reducible_valid _) red).
+    pose proof (iffRL (STLCmu_prim_red _) H).
+    destruct H0 as [e'' Hstep'].
+    by eapply proj_expr_step_help.
+  }
+  apply proj_expr_Reducible.
+  apply STLCmuVS.reducibility.Reducible_valid.
+  apply STLCmuVS_prim_red. by exists e'.
+Qed.
+
+Definition STLCmuVS_step_typed : relation STLCmuVS.lang.expr :=
+  fun e e' => STLCmuVS_step e e' ∧ (∃ Γ τ, STLCmuVS.typing.typed Γ e τ ∧ STLCmuVS.typing.typed Γ e' τ).
+
+Lemma rtc_STLCmuVS_step_typed (e e' : STLCmuVS.lang.expr) Γ τ (de : STLCmuVS.typing.typed Γ e τ) :
+  rtc STLCmuVS_step e e' → rtc STLCmuVS_step_typed e e'.
+Proof.
+  intro rtc. revert Γ τ de. induction rtc.
+  - constructor.
+  - intros. eapply rtc_l. repeat split. apply H. exists Γ, τ.
+    split; auto.
+    eapply preservation; eauto. apply reducibility.Reducible_valid. apply STLCmuVS_prim_red. by eexists.
+    eapply IHrtc.
+    eapply preservation; eauto. apply reducibility.Reducible_valid. apply STLCmuVS_prim_red. by eexists.
+Qed.
+
+Lemma proj_expr_halts (e : STLCmuVS.lang.expr) Γ τ (de : STLCmuVS.typing.typed Γ e τ) :
+  STLCmuVS_halts e → STLCmu_halts (proj_expr e).
+Proof.
+  intros halts. destruct halts as [v Hrtc].
+  exists (proj_val v). rewrite of_val_proj_expr.
+  assert (rtc STLCmuVS_step_typed e v).
+  { eapply rtc_subrel. eauto.
+    eapply rtc_STLCmuVS_step_typed; eauto.
+  }
+  eapply rtc_congruence; [|apply H].
+  intros e' e'' (Hstep & (Γ' & τ' & [de' de''])).
+  eapply proj_expr_step; eauto.
+Qed.
+
+Lemma inverse (e : STLCmuVS.lang.expr) Γ τ (de : STLCmuVS.typing.typed Γ e τ) :
+  embd_expr (proj_expr e) = e.
+Proof. induction de; simpl; (try done); (try by rewrite IHde1 IHde2); (try by rewrite IHde1 IHde2 IHde3); (try by rewrite IHde). Qed.
+
+Lemma proj_expr_halts' (e : STLCmuVS.lang.expr) Γ τ (de : STLCmuVS.typing.typed Γ e τ) :
+  STLCmu_halts (proj_expr e) → STLCmuVS_halts e.
+Proof.
+  intros halts. pose proof (embd_expr_halts _ halts) as halts'.
+  erewrite inverse in halts'; eauto.
+Qed.
+
+Lemma proj_expr_halts_iff (e : STLCmuVS.lang.expr) Γ τ (de : STLCmuVS.typing.typed Γ e τ) :
+  STLCmuVS_halts e <-> STLCmu_halts (proj_expr e).
+Proof. split; [by eapply proj_expr_halts | by eapply proj_expr_halts']. Qed.
+
+(* composing (STLCmu → STLCmuVS) with (STLCmuVS → STLCmuST) gives (STLCmu → STLCmuST) *)
+(* ---------------------------------------------------------------------------------- *)
+
+From st.embedding Require expressions contexts.
+From st.end_to_end Require embedding_STLCmu_STLCmuST.
+
+Lemma comp_embeddings (e : STLCmu.lang.expr) :
+  embedding.expressions.embd_expr (embd_expr e) = embedding_STLCmu_STLCmuST.embd_expr e.
+Proof. induction e; by simpl; repeat f_equiv; (try destruct (_ : base_lit)). Qed.
