theories/end_to_end/back_ctx_STLCmuST_STLCmu.v
@@ -1,0 +1,45 @@
+From st.STLCmuST Require Import lang types typing.
+From st.STLCmu Require Import types lang typing contexts.
+From st.STLCmuST Require Import contexts.
+From st.embedding Require Import types.
+From st.thms Require Import back_ctx_st_syn.
+From st.STLCmu Require Import boring.
+From st.end_to_end Require Import embedding_STLCmu_STLCmuST.
+From st.STLCmuVS Require Import lang.
+
+Section back_ctx_STLCmuST_STLCmu.
+
+  (* Given any syntactically-typed context in STLCmuST, ⊢ₛₜ C : ([[Γ]];[[τ]]) ⇒ ([];1), *)
+  Context (C : ctx)
+          (Γ : list type) (pΓ : Forall Closed Γ) (τ : type) (pτ : Closed τ)
+          (pC : typed_ctx C (embed <$> Γ) (embed τ) [] (embed TUnit)).
+
+  (* we have a syntactically typed context in STLCmu, C_b, *)
+  Definition back_ctx_STLCmuST_STLCmu : STLCmu.contexts.ctx :=
+    proj_ctx (back_ctx_st_syn C Γ τ).
+
+  (* It is indeed syntactically typed of (Γ;τ) ⇒ ([];1) *)
+  Lemma back_ctx_STLCmuST_STLCmu_typed :
+    STLCmu.contexts.typed_ctx back_ctx_STLCmuST_STLCmu Γ τ [] TUnit.
+  Proof. by apply proj_ctx_typed, back_ctx_st_syn_syn_typed. Qed.
+
+  (* Furthermore, the backtranslated contexts successfully emulates the original (when interacting with syntactically typed terms in STLCmu). *)
+  (* That is, for all syntactically typed e, Γ ⊢ₙₒ e : τ, C_b[e]⇓ ⇔ C[[[e]]]⇓ *)
+
+  Lemma back_ctx_STLCmuST_STLCmu_correct_emulation :
+    ∀ (e : STLCmu.lang.expr) (de : Γ ⊢ₙₒ e : τ),
+      STLCmu_halts (STLCmu.contexts.fill_ctx back_ctx_STLCmuST_STLCmu e) <-> STLCmuST_halts (fill_ctx C (embd_expr e)).
+  Proof.
+    intros e de.
+    rewrite -(comp_embeddings e).
+    rewrite /back_ctx_STLCmuST_STLCmu.
+    rewrite -(retraction e).
+    erewrite comm_proj_fill_ctx; [ |apply back_ctx_st_syn_syn_typed; eauto].
+    apply (@iff_trans _ (STLCmuVS_halts (contexts.fill_ctx (back_ctx_st_syn C Γ τ) (boring.embd_expr e))) _).
+    - apply iff_sym. apply (proj_expr_halts_iff (contexts.fill_ctx (back_ctx_st_syn C Γ τ) (boring.embd_expr e)) [] TUnit).
+      eapply contexts.typed_ctx_typed; [by apply boring.embd_expr_typed| apply back_ctx_st_syn_syn_typed; auto].
+    - rewrite (retraction e). apply back_ctx_st_syn_correct_emulation; auto.
+      by apply boring.embd_expr_typed.
+  Qed.
+
+End back_ctx_STLCmuST_STLCmu.
