theories/end_to_end/pres_ctx_equiv.v
@@ -1,0 +1,39 @@
+From st.thms Require Import back_ctx_st_syn.
+From st.STLCmu Require Import types lang typing contexts.
+From st.STLCmuST Require Import lang types typing contexts.
+From st.embedding Require Import types typed.
+From st.STLCmu Require Import boring.
+From st.end_to_end Require Import embedding_STLCmu_STLCmuST back_ctx_STLCmuST_STLCmu.
+
+Definition STLCmu_equiv Γ e1 e2 τ :=
+  Forall Closed Γ ∧ Closed τ ∧
+  Γ ⊢ₙₒ e1 : τ ∧ Γ ⊢ₙₒ e2 : τ ∧
+  ∀ C (dC : STLCmu.contexts.typed_ctx C Γ τ [] STLCmu.types.TUnit),
+    STLCmu_halts (STLCmu.contexts.fill_ctx C e1) <-> STLCmu_halts (STLCmu.contexts.fill_ctx C e2).
+
+Definition STLCmuST_equiv (Γ : list type) e1 e2 (τ : type) :=
+  Forall Closed Γ ∧ Closed τ ∧
+  Γ ⊢ₛₜ e1 : τ ∧ Γ ⊢ₛₜ e2 : τ ∧
+  ∀ C (dC : STLCmuST.contexts.typed_ctx C Γ τ [] STLCmuST.types.TUnit),
+    STLCmuST_halts (STLCmuST.contexts.fill_ctx C e1) <-> STLCmuST_halts (STLCmuST.contexts.fill_ctx C e2).
+
+Theorem preservation_STLCmu_equiv Γ e1 e2 τ :
+  STLCmu_equiv Γ e1 e2 τ → STLCmuST_equiv (embed <$> Γ) [[e1]] [[e2]] (embed τ).
+Proof.
+  intros (dΓ & dτ & de1 & de2 & Hequiv).
+  repeat split.
+  (* bookkeeping *)
+  eapply Forall_fmap, Forall_impl; eauto. intros. by apply embed_pres_closed.
+  by apply embed_pres_closed.
+  by rewrite -comp_embeddings; apply embd_typed, boring.embd_expr_typed.
+  by rewrite -comp_embeddings; apply embd_typed, boring.embd_expr_typed.
+  (* okay *)
+  - intro Halts.
+    eapply back_ctx_STLCmuST_STLCmu_correct_emulation; eauto.
+    apply Hequiv; first by apply back_ctx_STLCmuST_STLCmu_typed.
+    eapply back_ctx_STLCmuST_STLCmu_correct_emulation; eauto.
+  - intro SynHalts.
+    eapply back_ctx_STLCmuST_STLCmu_correct_emulation; eauto.
+    apply Hequiv; first by apply back_ctx_STLCmuST_STLCmu_typed.
+    eapply back_ctx_STLCmuST_STLCmu_correct_emulation; eauto.
+Qed.
