theories/prelude/lang_base.v
@@ -1,0 +1,8 @@
+From st.prelude Require Export generic.
+
+Inductive base_lit : Set :=
+| LitInt (n : Z) | LitBool (b : bool) | LitUnit.
+
+Inductive bin_op : Set :=
+| PlusOp | MinusOp | LeOp | LtOp | EqOp.
+
